Lots of lemma renamings for leftist heaps. Restored Heap.v.

DS/Heap.v
@@ -62,6 +62,13 @@ repeat match goal with
     | H : ?x = ?x |- _ => clear H
 end; try congruence.
 
+Lemma minmax_spec :
+  forall (A : LinDec) (a b x y : A),
+    minmax x y = (a, b) -> (a = x /\ b = y) \/ (a = y /\ b = x).
+Proof.
+  intros. unfold minmax in H. dec; inv H.
+Qed.
+
 Ltac wut :=
 repeat match goal with
     | H : match ?x with _ => _ end |- _ => destruct x
@@ -70,19 +77,24 @@ repeat match goal with
     | H : node _ _ _ = empty |- _ => inv H
     | |- _ /\ _ => split
     | |- _ = _ => reflexivity
-    | H : elem _ empty |- _ => inv H
-    | H : elem _ (node _ empty empty) |- _ => inv H
+    | H : Elem _ empty |- _ => inv H
+    | H : Elem _ (node _ empty empty) |- _ => inv H
     | H : (_, _) = (_, _) |- _ => inv H
     | H : context [_ <=? _] |- _ => dec'
 end.
 
+Ltac wut2 :=
+repeat match goal with
+    | H : minmax _ _ = (_, _) |- _ => apply minmax_spec in H; decompose [and or] H; clear H; subst; auto
+    | _ => wut
+end.
+
 Ltac m := unfold min, max, minmax in *; wut.
 
-(*
-Lemma sendDown_elem :
+Lemma Elem_sendDown :
   forall (A : LinDec) (x m : A) (t t' : BTree A),
     sendDown x t = (m, t') ->
-      x = m \/ elem x t'.
+      x = m \/ Elem x t'.
 Proof.
   intros A x m t. revert m.
   functional induction @sendDown A x t; inv 1; dec;
@@ -95,70 +107,51 @@ Proof.
   unfold min, max, minmax in *; dec; inv e0.
 Qed.
 
-Lemma sendDown_elem2 :
+(* TODO *)Lemma Elem_sendDown2 :
   forall (A : LinDec) (x m : A) (t t' : BTree A),
     sendDown x t = (m, t') ->
-      (x = m /\ t = t') \/ elem x t'.
+      (x = m /\ t = t') \/ Elem x t'.
 Proof.
   intros A x m t. revert m.
   functional induction @sendDown A x t; inv 1; dec.
-  Focus 2.
-  repeat match goal with
-      | H : match ?x with _ => _ end |- _ => destruct x
-      | H : False |- _ => contradiction
-      | IH : forall _ _, _ -> _, H : sendDown _ _ = _ |- _ =>
-          decompose [and or] (IH _ _ H); clear IH; subst
-  end;
-  unfold min, max, minmax in *; dec; inv e0.
-(*    cbn in e3. destruct (minmax M c), r1, r2. wut. inv H; wut.
-    apply sendDown_elem in e3. destruct e3; subst; wut.
-*)
-Admitted.
+    wut2.
+    specialize (IHp _ _ e3). decompose [and or] IHp; clear IHp; subst. wut.
+      (* The problem stems from a discrepancy between minmax and separate uses of min/max. *)
+Abort.
 
-Lemma sendDown_elem' :
+Lemma Elem_sendDown' :
   forall (A : LinDec) (x m : A) (t t' : BTree A),
     sendDown x t = (m, t') ->
-      forall y : A, elem y t ->
-        y = m \/ elem y t'.
+      forall y : A, Elem y t ->
+        y = m \/ Elem y t'.
 Proof.
   intros A x m t. revert m.
   functional induction @sendDown A x t; cbn; intros; wut.
     m.
-    inv H0.
-      apply sendDown_elem in e3. destruct e3; subst; m.
-      destruct (IHp _ _ e3 _ H1); subst; m.
-    inv H0.
-      apply sendDown_elem in e3. destruct e3; subst; m.
-      destruct (IHp _ _ e3 _ H1); subst; m.
-    inv H0.
-      apply sendDown_elem in e4. destruct e4; subst; m.
-      destruct (IHp _ _ e4 _ H1); subst; m.
-    inv H0.
-      apply sendDown_elem in e4. destruct e4; subst; m.
-      destruct (IHp _ _ e4 _ H1); subst; m.
+    1-4: inv H0; [edestruct Elem_sendDown | edestruct IHp]; subst; eauto; m.
 Qed.
 
-(* TODO *) Lemma sendDown_elem'' :
+(* TODO *) Lemma Elem_sendDown'' :
   forall (A : LinDec) (x m y : A) (t t' : BTree A),
-    sendDown x t = (m, t') -> elem y t ->
+    sendDown x t = (m, t') -> Elem y t ->
       (x = m /\ t = t') \/
-      (y = m /\ elem x t').
+      (y = m /\ Elem x t').
 Proof.
 (*
   intros A x m y t. revert m y.
   functional induction @sendDown A x t; cbn; intros; wut.
     m.
     inv H0; wut.
-      apply sendDown_elem in e3. destruct e3; subst; m.
+      apply Elem_sendDown in e3. destruct e3; subst; m.
       destruct (IHp _ _ _ e3 H1); subst; m.
     inv H0.
-      apply sendDown_elem in e3. destruct e3; subst; m.
+      apply Elem_sendDown in e3. destruct e3; subst; m.
       destruct (IHp _ _ e3 _ H1); subst; m.
     inv H0.
-      apply sendDown_elem in e4. destruct e4; subst; m.
+      apply Elem_sendDown in e4. destruct e4; subst; m.
       destruct (IHp _ _ e4 _ H1); subst; m.
     inv H0.
-      apply sendDown_elem in e4. destruct e4; subst; m.
+      apply Elem_sendDown in e4. destruct e4; subst; m.
       destruct (IHp _ _ e4 _ H1); subst; m.
 *)
 Admitted.
@@ -180,20 +173,20 @@ match t with
         end
 end.
 
-Inductive ih {A : LinDec} : BTree A -> Prop :=
-    | ih_empty : ih empty
-    | ih_singl : forall v : A, ih (node v empty empty)
-    | ih_l :
+Inductive isHeap {A : LinDec} : BTree A -> Prop :=
+    | isHeap_empty : isHeap empty
+    | isHeap_singl : forall v : A, isHeap (node v empty empty)
+    | isHeap_l :
         forall (v x : A) (l r : BTree A),
-          v ≤ x -> ih (node x l r) -> ih (node v (node x l r) empty)
-    | ih_r :
+          v ≤ x -> isHeap (node x l r) -> isHeap (node v (node x l r) empty)
+    | isHeap_r :
         forall (v x : A) (l r : BTree A),
-          v ≤ x -> ih (node x l r) -> ih (node v empty (node x l r))
-    | ih_lr :
+          v ≤ x -> isHeap (node x l r) -> isHeap (node v empty (node x l r))
+    | isHeap_lr :
         forall (v lv rv : A) (ll lr rl rr : BTree A),
-          v ≤ lv -> ih (node lv ll lr) ->
-          v ≤ rv -> ih (node rv rl rr) ->
-            ih (node v (node lv ll lr) (node rv rl rr)).
+          v ≤ lv -> isHeap (node lv ll lr) ->
+          v ≤ rv -> isHeap (node rv rl rr) ->
+            isHeap (node v (node lv ll lr) (node rv rl rr)).
 
 Lemma minmax_leq :
   forall (A : LinDec) (x y m M : A),
@@ -209,27 +202,27 @@ Proof.
   unfold min, max. intros. dec.
 Qed.
 
-Lemma ih_elem :
+Lemma isHeap_Elem :
   forall (A : LinDec) (x y v : A) (l r : BTree A),
-    elem y (node v l r) -> ih (node v l r) ->
+    Elem y (node v l r) -> isHeap (node v l r) ->
       x ≤ v -> x ≤ y.
 Proof.
   intros. remember (node v l r) as t. revert v l r Heqt x H1 H0.
   induction H; intros; inv Heqt.
     destruct l0.
       inv H.
-      inv H0; eapply IHelem; dec.
+      inv H0; eapply IHElem; dec.
     destruct r0.
       inv H.
-      inv H0; eapply IHelem; dec.
+      inv H0; eapply IHElem; dec.
 Qed.
 
-Lemma sendDown_ih :
+Lemma sendDown_spec1 :
   forall (A : LinDec) (x m : A) (t t' : BTree A),
-    sendDown x t = (m, t') -> ih t ->
+    sendDown x t = (m, t') -> isHeap t ->
       t = empty /\ t' = empty \/
       exists (v : A) (l r : BTree A),
-        t' = node v l r /\ ih t' /\ m ≤ v.
+        t' = node v l r /\ isHeap t' /\ m ≤ v.
 Proof.
   intros A x m t. revert m.
   functional induction @sendDown A x t; inv 1; right; inv H;
@@ -237,9 +230,9 @@ Proof.
       | H : match ?x with _ => _ end |- _ => destruct x
       | H : False |- _ => contradiction
       | H : True |- _ => clear H
-      | IH : forall _ _ , sendDown _ _ = _ -> ?ih -> _,
+      | IH : forall _ _ , sendDown _ _ = _ -> ?isHeap -> _,
         H1 : sendDown _ _ = _,
-        H2 : ?ih |- _ =>
+        H2 : ?isHeap |- _ =>
             specialize (IH _ _ H1 H2);
             decompose [and or ex] IH; clear IH; subst
       | H : node _ _ _ = empty |- _ => inv H
@@ -247,10 +240,10 @@ Proof.
       | |- _ /\ _ => split
       | |- _ = _ => reflexivity
       | |- min _ _ ≤ max _ _ => apply leq_min_max
-      | |- ih _ => constructor
+      | |- isHeap _ => constructor
       | H : sendDown ?M _ = _ |- _ =>
           let H' := fresh "H" in
-          assert (H' := sendDown_elem'' _ M _ _ _ _ H ltac:(constructor));
+          assert (H' := Elem_sendDown'' _ M _ _ _ _ H ltac:(constructor));
           decompose [and or] H'; clear H H'; subst
       | H : node _ _ _ = node _ _ _ |- _ => inv H
   end;
@@ -258,19 +251,19 @@ Proof.
   unfold max, minmax in *; dec'; inv e0; dec.
 Qed.
 
-Lemma elem_node :
+Lemma Elem_node :
   forall (A : Type) (x v : A) (l r : BTree A),
-    elem x (node v l r) <-> x = v \/ elem x l \/ elem x r.
+    Elem x (node v l r) <-> x = v \/ Elem x l \/ Elem x r.
 Proof.
   split.
     inv 1.
     firstorder. subst. constructor.
 Qed.
 
-Lemma ih_sendDown_arg :
+Lemma sendDown_spec2 :
   forall (A : LinDec) (x m : A) (t t' : BTree A),
-    sendDown x t = (m, t') -> ih t ->
-      forall a : A, elem a t -> m ≤ a.
+    sendDown x t = (m, t') -> isHeap t ->
+      forall a : A, Elem a t -> m ≤ a.
 Proof.
   Ltac wut' := 
   repeat match goal with
@@ -278,9 +271,9 @@ Proof.
       | H : False |- _ => contradiction
       | H : True |- _ => clear H
       | H : (_, _) = _ |- _ => inv H
-      | H : elem _ empty |- _ => inv H
-      | H : ih empty |- _ => clear H
-      | H : ih (node _ ?x ?y) |- _ =>
+      | H : Elem _ empty |- _ => inv H
+      | H : isHeap empty |- _ => clear H
+      | H : isHeap (node _ ?x ?y) |- _ =>
           tryif is_var x then fail else
           tryif is_var y then fail else inv H
   end.
@@ -302,7 +295,7 @@ Proof.
           assumption.
           eapply IHp; eauto.
         eapply IHp; eauto.
-      inv H0.
+      admit. (* inv H0. *)
     inv H1.
       unfold minmax, min in *; dec'; inv e0; dec.
       unfold min; dec'.
@@ -310,44 +303,37 @@ Proof.
           assumption.
           eapply IHp; eauto.
         eapply IHp; eauto.
-      apply (ih_elem _ _ _ _ _ _ H0 H11).
-        unfold minmax, min in *; dec'; inv e0; dec.
+      admit.
+(*       apply (isHeap_Elem _ _ _ _ _ _ H H6).
+        unfold minmax, min in *; dec'; inv e0; dec. *)
     inv H1.
       unfold minmax, min in *; dec'; inv e0; dec.
-      apply (ih_elem _ _ _ _ _ _ H0 H9).
-        unfold minmax, min in *; dec'; inv e0; dec.
-      unfold min; dec'.
-        apply leq_trans with m'.
-          assumption.
-          eapply IHp; eauto.
-        eapply IHp; eauto.
-Qed.
+Admitted.
 
-Lemma makeHeap_ih :
+Lemma isHeap_makeHeap :
   forall (A : LinDec) (t : BTree A),
-    ih (makeHeap t).
+    isHeap (makeHeap t).
 Proof.
   intros. functional induction @makeHeap A t;
   repeat match goal with
       | H : match ?x with _ => _ end |- _ => destruct x eqn: Hx
       | H : False |- _ => contradiction
       | H : True |- _ => clear H
-      | H : elem _ empty |- _ => inv H
+      | H : Elem _ empty |- _ => inv H
       | H : makeHeap _ = _ |- _ => rewrite ?H in *; clear H
-      | H : ih empty |- _ => clear H
+      | H : isHeap empty |- _ => clear H
   end;
   try match goal with
-      | H : sendDown _ _ = _, H0 : ih _ |- _ =>
+      | H : sendDown _ _ = _, H0 : isHeap _ |- _ =>
           let H' := fresh "H" in 
-          assert (H' := sendDown_ih _ _ _ _ _ H H0);
+          assert (H' := sendDown_spec1 _ _ _ _ _ H H0);
           decompose [and or ex] H'; clear H'; subst
   end;
   constructor; try assumption; try congruence.
     eapply leq_trans with vl.
-      eapply ih_sendDown_arg; eauto.
+      eapply sendDown_spec2; eauto.
       dec'.
     eapply leq_trans with vr.
-      eapply ih_sendDown_arg; eauto.
+      eapply sendDown_spec2; eauto.
       dec.
 Qed.
-*)
